operations/BMV_Fixpoint.thy
@@ -3,9 +3,10 @@ theory BMV_Fixpoint
 begin
 
 type_synonym ('tv, 'v, 'btv, 'bv, 'c, 'd) FTerm_pre' =
-  "'v                    \<comment>\<open>Var 'v\<close>
-  + 'd * 'd              \<comment>\<open>App \<open>('tv, 'v) FTerm\<close> \<open>('tv, 'v) FTerm\<close>\<close>
-  + 'd * 'tv FType       \<comment>\<open>TyApp \<open>('tv, 'v) FTerm\<close> \<open>'tv FType\<close>\<close>
+  "('v                    \<comment>\<open>Var 'v\<close>
+  + 'd * 'd               \<comment>\<open>App \<open>('tv, 'v) FTerm\<close> \<open>('tv, 'v) FTerm\<close>\<close>
+  \<comment>\<open>+ 'v list\<close>
+  ) + 'd * 'tv FType       \<comment>\<open>TyApp \<open>('tv, 'v) FTerm\<close> \<open>'tv FType\<close>\<close>
   + 'bv * 'tv FType * 'c \<comment>\<open>Lam x::'v \<open>'tv FType\<close> t::\<open>('tv, 'v) FTerm\<close> binds x in t\<close>
   + 'btv * 'c            \<comment>\<open>TyLam a::'tv t::\<open>('tv, 'v) FTerm\<close> binds a in t\<close>"
 
@@ -15,17 +16,18 @@ ML \<open>
 Multithreading.parallel_proofs := 0
 \<close>
 
+declare [[mrbnf_internals=false]]
 local_setup \<open>fn lthy =>
 let
   val T = @{typ "('tv, 'v, 'btv, 'bv, 'c, 'd) FTerm_pre'"};
   val Xs = [@{typ 'tv}, @{typ 'v}, @{typ 'btv}, @{typ 'bv}, @{typ 'c}, @{typ 'd}];
 
-  val ((mrsbnf, (Ds, tys)), ((bmv_unfolds, (_, mrbnf_unfolds)), lthy)) = MRSBNF_Comp.mrsbnf_of_typ true (K BNF_Def.Dont_Note)
+  val ((mrsbnf, (Ds, tys)), (((_, bmv_unfolds), (_, mrbnf_unfolds)), lthy)) = MRSBNF_Comp.mrsbnf_of_typ true (K BNF_Def.Dont_Note)
     I [] (map (apfst dest_TFree) [(@{typ 'v}, MRBNF_Def.Free_Var),
       (@{typ 'btv}, MRBNF_Def.Bound_Var), (@{typ 'bv}, MRBNF_Def.Bound_Var)])
     (fn xss => inter (op=) (flat xss) (map dest_TFree Xs))
     T
-    (([], (MRBNF_Comp.empty_comp_cache, MRBNF_Comp.empty_unfolds)), lthy);
+    (((Symtab.empty, []), (MRBNF_Comp.empty_comp_cache, MRBNF_Comp.empty_unfolds)), lthy);
 
   val mrsbnf = case mrsbnf of MRBNF_Util.Inl x => x | _ => error "impossible"
 
@@ -60,24 +62,42 @@ let
   (* Step 5: Define recursor locales *)  
   val (recursor_result, lthy) = MRBNF_Recursor.create_binding_recursor I fp_res lthy;
 
-  (*val ([(rec_mrbnf, vvsubst_res)], lthy) = MRBNF_VVSubst.mrbnf_of_quotient_fixpoint [@{binding vvsubst_FTerm}]
+  val ([(rec_mrbnf, vvsubst_res)], lthy) = MRBNF_VVSubst.mrbnf_of_quotient_fixpoint [@{binding vvsubst_FTerm}]
     I fp_res (#QREC_fixed recursor_result) lthy;
   val lthy = MRBNF_Def.register_mrbnf_raw (fst (dest_Type (#T (hd (#quotient_fps fp_res))))) rec_mrbnf lthy;
-  *)
+
 in lthy end
 \<close>
 print_theorems
 
+thm bmv_defs
+
 (* Substitution axioms *)
 abbreviation \<eta> :: "'v::var \<Rightarrow> ('tv::var, 'v::var, 'a::var, 'b::var, 'c, 'd) FTerm_pre" where
-  "\<eta> a \<equiv> Abs_FTerm_pre (Inl a)"
+  "\<eta> a \<equiv> Abs_FTerm_pre (Inl (Inl a))"
 
-lemma eta_free: "set2_FTerm_pre (\<eta> a) = {a}"
+(* Because RVrs is completely overwritten *)
+lemma eta_free: "RVrs_FTerm_pre (\<eta> a) = {a}"
   apply (unfold set2_FTerm_pre_def sum.set_map UN_empty2 Un_empty_left Un_empty_right prod.set_map comp_def
-    Abs_FTerm_pre_inverse[OF UNIV_I] sum_set_simps UN_empty UN_single
+    Abs_FTerm_pre_inverse[OF UNIV_I] sum_set_simps UN_empty UN_single RVrs_FTerm_pre_def bmv_defs
   )
   apply (rule refl)
   done
+lemma eta_compl_free: "\<forall>a. x \<noteq> \<eta> a \<Longrightarrow> RVrs_FTerm_pre x = {}"
+  apply (tactic \<open>resolve_tac @{context} [infer_instantiate' @{context} [SOME @{cterm x}] (
+    BNF_FP_Util.mk_absumprodE @{thm type_definition_FTerm_pre} [1, 2, 2, 3, 2]
+  )] 1\<close>; hypsubst_thin)
+   apply (unfold Sb_FTerm_pre_def comp_def Abs_FTerm_pre_inject[OF UNIV_I UNIV_I] bmv_defs Abs_FTerm_pre_inverse[OF UNIV_I]
+      map_sum.simps Map_FTerm_pre_def sum.inject RVrs_FTerm_pre_def bmv_defs sum_set_simps UN_single cSup_singleton
+      Union_empty Un_empty_right UN_empty
+    )
+  apply (erule contrapos_pp)
+      apply (unfold not_all not_not)
+      apply (rule exI)
+      apply (rule refl)+
+  done
+
+
 lemma eta_inj: "\<eta> a = \<eta> b \<Longrightarrow> a = b"
   apply (unfold Abs_FTerm_pre_inject[OF UNIV_I UNIV_I] sum.inject)
   apply assumption
@@ -90,6 +110,20 @@ lemma eta_natural:
   apply (rule ext)
   apply (unfold comp_def map_FTerm_pre_def Abs_FTerm_pre_inverse[OF UNIV_I] map_sum.simps)
   apply (rule refl)
+  done
+
+lemma eta_Sb:
+  fixes x::"('tv::var, 'v::var, 'c::var, 'd::var, 'e, 'f) FTerm_pre"
+  assumes "|supp f| <o |UNIV::'v set|" "|SSupp TyVar \<rho>| <o |UNIV::'tv set|"
+  shows "Sb_FTerm_pre f \<rho> (Map_FTerm_pre h1 h2 x) = \<eta> a \<Longrightarrow> \<exists>a. x = \<eta> a"
+  apply (tactic \<open>resolve_tac @{context} [infer_instantiate' @{context} [SOME @{cterm x}] (
+    BNF_FP_Util.mk_absumprodE @{thm type_definition_FTerm_pre} [1, 2, 2, 3, 2]
+  )] 1\<close>; hypsubst_thin)
+      apply (unfold Sb_FTerm_pre_def comp_def Abs_FTerm_pre_inject[OF UNIV_I UNIV_I] bmv_defs Abs_FTerm_pre_inverse[OF UNIV_I]
+      map_sum.simps Map_FTerm_pre_def)
+      apply (rule exI, rule refl)
+    (* orelse *)
+     apply (((unfold sum.inject)[1])?, erule sum.distinct[THEN notE])+
   done
 
 (* Construction of substitution *)
@@ -373,11 +407,39 @@ lemma eta_set_empties:
     done
   done
 
+lemma not_is_VVr_Sb:
+  fixes x::"('tv::var, 'v::var, 'tv, 'v, ('tv, 'v) FTerm, ('tv, 'v) FTerm) FTerm_pre"
+  assumes "|supp f| <o |UNIV::'v set|" "|SSupp TyVar \<rho>| <o |UNIV::'tv set|"
+  shows "\<not>isVVr (FTerm_ctor x) \<Longrightarrow> \<not>isVVr (FTerm_ctor (Sb_FTerm_pre f \<rho> (Map_FTerm_pre h1 h2 x)))"
+  apply (unfold isVVr_def VVr_def comp_def)
+  apply (erule contrapos_nn)
+  apply (erule exE)
+  apply (subst (asm) FTerm.TT_inject0)
+  apply (erule exE conjE)+
+  subgoal for a f1 f2
+    apply (drule arg_cong[of _ _ "map_FTerm_pre id id (inv f1) (inv f2) (permute_FTerm (inv f1) (inv f2)) id"])
+    apply (subst (asm) FTerm_pre.map_comp)
+              apply (rule supp_id_bound bij_id bij_imp_bij_inv supp_inv_bound | assumption)+
+    apply (subst (asm) FTerm.permute_comp0, (rule supp_id_bound bij_id bij_imp_bij_inv supp_inv_bound | assumption)+)+
+    apply (unfold id_o o_id inv_o_simp1 FTerm.permute_id0 FTerm_pre.map_id)
+    apply (subst (asm) eta_natural[THEN fun_cong, unfolded comp_def])
+          apply (rule supp_id_bound bij_id bij_imp_bij_inv supp_inv_bound | assumption)+
+    apply (drule eta_Sb[OF assms])
+    apply (erule exE)
+    apply hypsubst_thin
+    apply (rule exI)
+    apply (rule refl)
+    done
+  done
+
 lemmas Cinfinite_UNIV = conjI[OF FTerm_pre.UNIV_cinfinite card_of_Card_order]
 lemmas Cinfinite_card = cmin_Cinfinite[OF Cinfinite_UNIV Cinfinite_UNIV]
 lemmas regularCard_card = cmin_regularCard[OF FTerm_pre.var_regular FTerm_pre.var_regular Cinfinite_UNIV Cinfinite_UNIV]
 lemmas Un_bound = regularCard_Un[OF conjunct2[OF Cinfinite_card] conjunct1[OF Cinfinite_card] regularCard_card]
 lemmas UN_bound = regularCard_UNION[OF conjunct2[OF Cinfinite_card] conjunct1[OF Cinfinite_card] regularCard_card]
+
+abbreviation (input) "avoiding_set1 f1 f2 \<equiv> IImsupp_FTerm1 f1 \<union> (SSupp TyVar f2 \<union> IImsupp TyVar FVars_FType f2)"
+abbreviation (input) "avoiding_set2 f1 \<equiv> SSupp VVr f1 \<union> IImsupp_FTerm2 f1"
 
 context
   fixes f1::"'var::var \<Rightarrow> ('tyvar::var, 'var) FTerm" and f2::"'tyvar \<Rightarrow> 'tyvar FType"
@@ -385,8 +447,8 @@ context
     "|SSupp TyVar f2| <o cmin |UNIV::'tyvar set| |UNIV::'var set|"
 begin
 
-interpretation tvsubst: QREC_cmin_fixed_FTerm "IImsupp_FTerm1 f1 \<union> (SSupp TyVar f2 \<union> IImsupp TyVar FVars_FType f2)"
-  "IImsupp_FTerm2 f1" "\<lambda>y. if isVVr (FTerm_ctor (map_FTerm_pre id id id id fst fst y)) then
+interpretation tvsubst: QREC_cmin_fixed_FTerm "avoiding_set1 f1 f2"
+  "avoiding_set2 f1" "\<lambda>y. if isVVr (FTerm_ctor (map_FTerm_pre id id id id fst fst y)) then
     f1 (asVVr (FTerm_ctor (map_FTerm_pre id id id id fst fst y)))
   else FTerm_ctor (Sb_FTerm_pre id f2 (map_FTerm_pre id id id id snd snd y))"
   apply unfold_locales
@@ -415,8 +477,9 @@ interpretation tvsubst: QREC_cmin_fixed_FTerm "IImsupp_FTerm1 f1 \<union> (SSupp
      apply (rule IImsupp_permute_commute[THEN fun_cong, unfolded comp_def])
           apply (assumption | rule ordLess_ordLeq_trans cmin1 cmin2 card_of_Card_order)+
       apply (erule Int_subset_empty2)
-      apply (rule subsetI)
-      apply (assumption | erule UnI1 UnI2 | rule UnI1)+
+    apply (rule Un_upper1)
+      apply (erule Int_subset_empty2)
+    apply (rule Un_upper1 Un_upper2)
 
     apply (rule trans)
     apply (rule FTerm.permute_ctor)
@@ -431,6 +494,7 @@ interpretation tvsubst: QREC_cmin_fixed_FTerm "IImsupp_FTerm1 f1 \<union> (SSupp
          apply (assumption  | erule ordLess_ordLeq_trans[OF _ cmin1] ordLess_ordLeq_trans[OF _ cmin2]
         | rule supp_id_bound card_of_Card_order supp_inv_bound SSupp_comp_bound infinite_UNIV FType.SSupp_map_bound
           f_prems[THEN ordLess_ordLeq_trans, OF cmin1] f_prems[THEN ordLess_ordLeq_trans, OF cmin2]
+           card_of_Card_order conjI cinfinite_iff_infinite[THEN iffD2]
         | (unfold comp_assoc)[1])+
      apply (rule refl)
     apply (subst (asm) FTerm_pre.map_comp, (assumption | erule ordLess_ordLeq_trans[OF _ cmin1] ordLess_ordLeq_trans[OF _ cmin2] | rule card_of_Card_order supp_id_bound bij_id)+)
@@ -545,9 +609,8 @@ interpretation tvsubst: QREC_cmin_fixed_FTerm "IImsupp_FTerm1 f1 \<union> (SSupp
        apply assumption
       apply (rule Un_upper1)
     apply (rule subsetI)
-     apply (rule UnI2)
+     apply (rule UnI2)+
      apply (unfold IImsupp_def SSupp_def)[1]
-    apply (rule UnI2)
      apply (rule UN_I)
       apply (rule CollectI)
       apply assumption
@@ -613,7 +676,7 @@ lemma tvsubst_VVr: "tvsubst_FTerm (VVr a) = f1 a"
   done
 
 lemma tvsubst_not_is_VVr:
-  assumes empty_prems: "set3_FTerm_pre x \<inter> (IImsupp_FTerm1 f1 \<union> (SSupp TyVar f2 \<union> IImsupp TyVar FVars_FType f2)) = {}" "set4_FTerm_pre x \<inter> IImsupp_FTerm2 f1 = {}"
+  assumes empty_prems: "set3_FTerm_pre x \<inter> avoiding_set1 f1 f2 = {}" "set4_FTerm_pre x \<inter> avoiding_set2 f1 = {}"
   and noclash: "noclash_FTerm x"
   and VVr_prems: "\<not>isVVr (FTerm_ctor x)"
   shows "tvsubst_FTerm (FTerm_ctor x) = FTerm_ctor (Sb_FTerm_pre id f2 (map_FTerm_pre id id id id tvsubst_FTerm tvsubst_FTerm x))"
@@ -627,6 +690,365 @@ lemma tvsubst_not_is_VVr:
   apply (rule assms)
   done
 end
+
+lemma eta_ctor_inj: "FTerm_ctor (\<eta> a) = FTerm_ctor x \<Longrightarrow> x = \<eta> a"
+  apply (unfold FTerm.TT_inject0)
+  apply (erule exE conjE)+
+  apply (subst (asm) eta_natural')
+        apply (rule supp_id_bound bij_id | assumption)+
+  apply (unfold id_apply)
+  apply (erule sym)
+  done
+
+lemma in_IImsupps:
+  "f1 a \<noteq> VVr a \<Longrightarrow> z \<in> FVars (f1 a) \<Longrightarrow> z \<in> IImsupp VVr FVars f1"
+  "f1 a \<noteq> VVr a \<Longrightarrow> z2 \<in> FTVars (f1 a) \<Longrightarrow> z2 \<in> IImsupp VVr FTVars f1"
+  apply (unfold IImsupp_def SSupp_def)
+  apply (rule UN_I)
+   apply (erule CollectI)
+  apply assumption
+  apply (rule UN_I)
+   apply (erule CollectI)
+  apply assumption
+  done
+
+lemma FVars_VVr:
+  "FVars (VVr a) = {a}"
+  "FTVars (VVr a) = {}"
+  apply (unfold VVr_def comp_def FTerm.FVars_ctor eta_set_empties UN_empty Diff_empty Un_empty_right FTerm_pre.set_Vrs)
+   apply (rule eta_free)
+  apply (unfold FTerm_pre.set_Vrs[symmetric])
+  apply (rule eta_set_empties)
+  done
+
+lemma IImsupp_Diff:
+  "B \<inter> avoiding_set2 f1 = {} \<Longrightarrow> (\<Union>a\<in>(A - B). FVars (f1 a)) = (\<Union>a\<in>A. FVars (f1 a)) - B"
+  "B \<inter> avoiding_set2 f1 = {} \<Longrightarrow> B2 \<inter> avoiding_set1 f1 f2 = {} \<Longrightarrow> (\<Union>a\<in>(A - B). FTVars (f1 a)) = (\<Union>a\<in>A. FTVars (f1 a)) - B2"
+  apply (rule set_eqI)
+  apply (rule iffI)
+    (* helper_tac false *)
+   apply (erule UN_E DiffE)+
+   apply (rule DiffI UN_I)+
+     apply assumption
+    apply assumption
+   apply (rule case_split[of "_ = _"])
+    (* apply (rotate_tac -2) *)
+    apply (drule iffD1[OF arg_cong2[OF refl, of _ _ "(\<in>)"], rotated])
+     apply (rule trans)
+      apply (rule arg_cong[of _ _ FVars])
+      apply assumption
+     apply (rule FVars_VVr)
+    apply (drule singletonD)
+    apply (rule iffD2[OF arg_cong2[OF _ refl, of _ _ "(\<notin>)"]])
+    (* apply (rule sym) *)
+     apply assumption
+    apply assumption
+   apply (frule in_IImsupps[rotated])
+    apply assumption
+   apply (drule trans[OF Int_commute])
+   apply (drule iffD1[OF disjoint_iff])
+   apply (erule allE)
+   apply (erule impE)
+    (* prefer 2 *)
+    apply (rule UnI2)+
+    apply assumption
+   apply assumption
+    (* END helper_tac false *)
+    (* helper_tac true *)
+  apply (erule UN_E DiffE)+
+  apply (rule DiffI UN_I)+
+    apply assumption
+    (*apply assumption*)
+   apply (rule case_split[of "_ = _"])
+    apply (rotate_tac -2)
+    apply (drule iffD1[OF arg_cong2[OF refl, of _ _ "(\<in>)"], rotated])
+     apply (rule trans)
+      apply (rule arg_cong[of _ _ FVars])
+      apply assumption
+     apply (rule FVars_VVr)
+    apply (drule singletonD)
+    apply (rule iffD2[OF arg_cong2[OF _ refl, of _ _ "(\<notin>)"], rotated])
+     apply assumption
+    apply (erule sym)
+   apply (frule in_IImsupps(1))
+    apply assumption
+   apply (drule trans[OF Int_commute])
+   apply (drule iffD1[OF disjoint_iff])
+   apply (erule allE)
+   apply (erule impE)
+    prefer 2
+    apply assumption
+    (* apply assumption *)
+    (* END helper_tac true *)
+   apply (unfold IImsupp_def SSupp_def)[1]
+   apply (rule UnI1)
+   apply (rule CollectI)
+   apply assumption
+   apply assumption
+(* second goal *)
+  apply (rule set_eqI)
+  apply (rule iffI)
+    (* helper_tac false *)
+   apply (erule UN_E DiffE)+
+   apply (rule DiffI UN_I)+
+     apply assumption
+    apply assumption
+   apply (rule case_split[of "_ = _"])
+    (* apply (rotate_tac -2) *)
+    apply (drule iffD1[OF arg_cong2[OF refl, of _ _ "(\<in>)"], rotated])
+     apply (rule trans)
+      apply (rule arg_cong[of _ _ FTVars])
+      apply assumption
+     apply (rule FVars_VVr)
+    apply (drule singletonD | erule emptyE)
+   apply (frule in_IImsupps[rotated])
+    apply assumption
+   apply (rotate_tac -1)
+   apply (erule disjoint_iff[THEN iffD1, THEN spec, THEN mp, rotated])
+   apply (rule trans[OF Int_commute])
+   apply (erule Int_subset_empty2)
+  apply (rule Un_upper1)
+    (* helper_tac true *)
+  apply (erule UN_E DiffE)+
+  apply (rule DiffI UN_I)+
+    apply assumption
+    (*apply assumption*)
+   apply (rule case_split[of "_ = _"])
+    apply (rotate_tac -2)
+    apply (drule iffD1[OF arg_cong2[OF refl, of _ _ "(\<in>)"], rotated])
+     apply (rule trans)
+      apply (rule arg_cong[of _ _ FTVars])
+      apply assumption
+     apply (rule FVars_VVr)
+    apply (drule singletonD | erule emptyE)
+   apply (frule in_IImsupps[rotated])
+    apply assumption
+   apply (erule disjoint_iff[THEN iffD1, THEN spec, THEN mp, OF trans[OF Int_commute]])
+    (* apply assumption *)
+    (* END helper_tac true *)
+   apply (unfold IImsupp_def SSupp_def)[1]
+   apply (rule UnI1)
+   apply (rule CollectI)
+   apply assumption
+   apply assumption
+  done
+
+lemma FVars_tvsubst1:
+  fixes f1::"'var::var \<Rightarrow> ('tyvar::var, 'var) FTerm" and f2::"'tyvar \<Rightarrow> 'tyvar FType"
+  assumes f_prems: "|SSupp VVr f1| <o cmin |UNIV::'tyvar set| |UNIV::'var set|"
+    "|SSupp TyVar f2| <o cmin |UNIV::'tyvar set| |UNIV::'var set|"
+  shows "FVars (tvsubst_FTerm f1 f2 t) = (\<Union>a\<in>FVars t. FVars (f1 a))"
+  apply (rule FTerm.TT_fresh_induct[of "avoiding_set1 f1 f2" "avoiding_set2 f1" _ t])
+  apply (unfold IImsupp_def)[2]
+    apply (rule var_class.Un_bound var_class.UN_bound cmin1 cmin2 card_of_Card_order FTerm.FVars_bd_UNIVs assms[THEN ordLess_ordLeq_trans]
+      FType.set_bd_UNIV
+    )+
+  apply (rule case_split[rotated])
+   apply (subst tvsubst_not_is_VVr[rotated -1])
+         apply assumption
+        apply (rule assms | assumption)+
+   apply (unfold FTerm.FVars_ctor)[1]
+   apply (subst FTerm_pre.set_Sb FTerm_pre.set_map, (rule supp_id_bound bij_id cmin1 cmin2 card_of_Card_order assms assms[THEN ordLess_ordLeq_trans])+)+
+   apply (unfold image_id FTerm_pre.set_Vrs(1-2) image_comp[unfolded comp_def] FTerm_pre.Map_map[symmetric])[1]
+   apply (subst FTerm_pre.Vrs_Sb, (rule supp_id_bound bij_id cmin1 cmin2 card_of_Card_order assms assms[THEN ordLess_ordLeq_trans])+)+
+   apply (unfold image_id FTerm_pre.Vrs_Map UN_Un)
+   apply (rule arg_cong2[of _ _ _ _ "(\<union>)"])+
+     apply (subst eta_compl_free)
+      apply (unfold isVVr_def)[1]
+      apply (rotate_tac -1)
+      apply (erule contrapos_np)
+      apply (unfold not_all not_not VVr_def comp_def)[1]
+      apply (erule exE)
+      apply hypsubst
+      apply (rule exI)
+  apply (rule refl)
+     apply (subst eta_compl_free)
+      apply (unfold isVVr_def)[1]
+      apply (rotate_tac -1)
+      apply (erule contrapos_np)
+      apply (unfold not_all not_not VVr_def comp_def)[1]
+      apply (erule exE)
+      apply hypsubst
+      apply (rule exI)
+      apply (rule refl)
+     apply (unfold UN_empty)
+     apply (rule refl)
+    apply (subst IImsupp_Diff)
+     apply assumption
+    apply (rule arg_cong2[OF _ refl, of _ _ "minus"])
+    apply (unfold UN_UN_flatten)
+    apply (rule UN_cong)
+    apply assumption
+
+   apply (rule UN_cong)
+   apply assumption
+
+  apply (unfold isVVr_def)
+  apply (erule exE)
+  apply (rotate_tac -1)
+  apply (erule subst[OF sym])
+  apply (subst tvsubst_VVr)
+    apply (rule assms)+
+  apply (unfold FVars_VVr UN_single)
+  apply (rule refl)
+  done
+
+lemma Un_forward: "a \<in> A \<union> B \<Longrightarrow> (a \<in> A \<Longrightarrow> a \<in> C) \<Longrightarrow> (a \<in> B \<Longrightarrow> a \<in> D) \<Longrightarrow> a \<in> C \<union> D"
+  by blast
+
+lemma Un_cong_FTVars: "A = A1 \<union> A2 \<Longrightarrow> B = B1 \<union> B2 \<Longrightarrow> C = C1 \<union> C2 \<Longrightarrow> A \<union> B \<union> C = (A1 \<union> B1 \<union> C1) \<union> (A2 \<union> B2 \<union> C2)"
+  apply hypsubst_thin
+  apply (rule set_eqI)
+  apply (rule iffI)
+   apply (erule UnE)
+    apply (erule UnE)
+    (* REPEAT_DETERM *)
+     apply (erule UnE)
+      apply (rule UnI1)
+      apply (tactic \<open>eresolve_tac @{context} [BNF_Util.mk_UnIN 3 1] 1\<close>)
+     apply (rule UnI2)
+     apply (tactic \<open>eresolve_tac @{context} [BNF_Util.mk_UnIN 3 1] 1\<close>)
+    (* repeated *)
+    apply (erule UnE)
+     apply (rule UnI1)
+     apply (tactic \<open>eresolve_tac @{context} [BNF_Util.mk_UnIN 3 2] 1\<close>)
+    apply (rule UnI2)
+    apply (tactic \<open>eresolve_tac @{context} [BNF_Util.mk_UnIN 3 2] 1\<close>)
+    (* repeated *)
+   apply (erule UnE)
+    apply (rule UnI1)
+    apply (tactic \<open>eresolve_tac @{context} [BNF_Util.mk_UnIN 3 3] 1\<close>)
+   apply (rule UnI2)
+   apply (tactic \<open>eresolve_tac @{context} [BNF_Util.mk_UnIN 3 3] 1\<close>)
+    (* END REPEAT_DETERM *)
+  apply (erule UnE)
+   apply (erule Un_forward)+
+     apply (erule UnI1)+
+  apply (erule Un_forward)+
+    apply (erule UnI2)+
+  done
+
+lemma FVars_tvsubst2:
+  fixes \<rho>1::"'var::var \<Rightarrow> ('tyvar::var, 'var) FTerm" and \<rho>2::"'tyvar \<Rightarrow> 'tyvar FType"
+  assumes f_prems: "|SSupp VVr \<rho>1| <o cmin |UNIV::'tyvar set| |UNIV::'var set|"
+    "|SSupp TyVar \<rho>2| <o cmin |UNIV::'tyvar set| |UNIV::'var set|"
+  shows "FTVars (tvsubst_FTerm \<rho>1 \<rho>2 t) = (\<Union>x\<in>FVars t. FTVars (\<rho>1 x)) \<union> (\<Union>x\<in>FTVars t. FVars_FType (\<rho>2 x))"
+  apply (rule FTerm.TT_fresh_induct[of "avoiding_set1 \<rho>1 \<rho>2" "avoiding_set2 \<rho>1" _ t])
+  apply (unfold IImsupp_def)[2]
+    apply (rule var_class.Un_bound var_class.UN_bound cmin1 cmin2 card_of_Card_order FTerm.FVars_bd_UNIVs assms[THEN ordLess_ordLeq_trans]
+      FType.set_bd_UNIV 
+    )+
+
+  apply (rule case_split[rotated])
+   apply (subst tvsubst_not_is_VVr[rotated -1])
+         apply assumption
+        apply (rule assms | assumption)+
+   apply (unfold FTerm.FVars_ctor)[1]
+   apply (subst FTerm_pre.set_Sb FTerm_pre.set_map, (rule supp_id_bound bij_id cmin1 cmin2 card_of_Card_order assms assms[THEN ordLess_ordLeq_trans])+)+
+   apply (unfold image_id FTerm_pre.set_Vrs(1-2) image_comp[unfolded comp_def] FTerm_pre.Map_map[symmetric])[1]
+   apply (subst FTerm_pre.Vrs_Sb, (rule supp_id_bound bij_id cmin1 cmin2 card_of_Card_order assms assms[THEN ordLess_ordLeq_trans])+)+
+   apply (unfold image_id FTerm_pre.Vrs_Map UN_Un)
+   apply (rule Un_cong_FTVars)
+     apply (subst eta_compl_free)
+      apply (unfold isVVr_def)[1]
+      apply (rotate_tac -1)
+      apply (erule contrapos_np)
+      apply (unfold not_all not_not VVr_def comp_def)[1]
+      apply (erule exE)
+      apply hypsubst
+      apply (rule exI)
+  apply (rule refl)
+     apply (unfold UN_empty Un_empty_left)
+     apply (rule refl)
+    apply (rule trans)
+     apply (rule arg_cong2[OF _ refl, of _ _ "minus"])
+     apply (rule UN_cong)
+     apply assumption
+
+    apply (subst IImsupp_Diff, assumption+)
+    apply (subst FType.IImsupp_Diff)
+     apply (erule Int_subset_empty2)
+  (* This is only because FType does not use BMVs yet, not part of the tactic *)
+     apply (unfold IImsupp_FType_def SSupp_FType_def tvVVr_tvsubst_FType_def tv\<eta>_FType_tvsubst_FType_def
+      TyVar_def[symmetric] SSupp_def[of TyVar, symmetric, THEN meta_eq_to_obj_eq, THEN fun_cong] 
+      comp_def IImsupp_def[of TyVar FVars_FType, symmetric, THEN meta_eq_to_obj_eq, THEN fun_cong]
+    )[1]
+     apply (rule Un_upper2)
+    apply (unfold Un_Diff[symmetric])
+    apply (rule arg_cong2[OF _ refl, of _ _ "minus"])
+    apply (unfold UN_UN_flatten UN_Un_distrib[symmetric])
+  apply (rule refl)
+
+   apply (rule UN_cong)
+   apply assumption
+
+  apply (unfold isVVr_def)
+  apply (erule exE)
+  apply (rotate_tac -1)
+  apply (erule subst[OF sym])
+  apply (subst tvsubst_VVr)
+    apply (rule assms)+
+  apply (unfold FVars_VVr UN_single UN_empty Un_empty_right)
+  apply (rule refl)
+  done
+lemmas FVars_tvsubst = FVars_tvsubst1 FVars_tvsubst2
+
+lemma SSupp_tvsubst_subset:
+  fixes \<rho>1::"'var::var \<Rightarrow> ('tyvar::var, 'var) FTerm" and \<rho>2::"'tyvar \<Rightarrow> 'tyvar FType"
+  assumes f_prems: "|SSupp VVr \<rho>1| <o cmin |UNIV::'tyvar set| |UNIV::'var set|"
+    "|SSupp TyVar \<rho>2| <o cmin |UNIV::'tyvar set| |UNIV::'var set|"
+  shows "SSupp VVr (tvsubst_FTerm \<rho>1 \<rho>2 \<circ> \<rho>1') \<subseteq> SSupp VVr \<rho>1 \<union> SSupp VVr \<rho>1'"
+  apply (rule subsetI)
+  apply (unfold SSupp_def mem_Collect_eq Un_iff de_Morgan_conj[symmetric])
+  apply (erule contrapos_nn)
+  apply (erule conjE)
+  apply (rule trans[OF comp_apply])
+  apply (rotate_tac)
+  apply (erule subst[OF sym])
+  apply (rule trans)
+   apply (rule tvsubst_VVr[OF assms])
+  apply assumption
+  done
+lemma SSupp_Sb_subset:
+  fixes \<rho>2::"'tyvar::var \<Rightarrow> 'tyvar FType"
+  assumes f_prems:
+    "|SSupp TyVar \<rho>2| <o cmin |UNIV::'tyvar set| |UNIV::'var set|"
+  shows "SSupp TyVar (tvsubst_FType \<rho>2 \<circ> \<rho>1') \<subseteq> SSupp TyVar \<rho>2 \<union> SSupp TyVar \<rho>1'"
+  apply (rule subsetI)
+  apply (unfold SSupp_def mem_Collect_eq Un_iff de_Morgan_conj[symmetric])
+  apply (erule contrapos_nn)
+  apply (erule conjE)
+  apply (rule trans[OF comp_apply])
+  apply (rotate_tac)
+  apply (erule subst[OF sym])
+  apply (rule trans)
+   apply (rule FType.Sb_comp_Inj[THEN fun_cong, unfolded comp_def])
+   apply (rule ordLess_ordLeq_trans)
+    apply (rule assms)
+   apply (rule cmin1 card_of_Card_order)+
+  apply assumption
+  done
+
+lemma SSupp_tvsubst_bound:
+  fixes \<rho>1::"'var::var \<Rightarrow> ('tyvar::var, 'var) FTerm" and \<rho>2::"'tyvar \<Rightarrow> 'tyvar FType"
+  assumes f_prems: "|SSupp VVr \<rho>1| <o cmin |UNIV::'tyvar set| |UNIV::'var set|"
+    "|SSupp TyVar \<rho>2| <o cmin |UNIV::'tyvar set| |UNIV::'var set|"
+    "|SSupp VVr \<rho>1'| <o cmin |UNIV::'tyvar set| |UNIV::'var set|"
+  shows "|SSupp VVr (tvsubst_FTerm \<rho>1 \<rho>2 \<circ> \<rho>1')| <o cmin |UNIV::'tyvar set| |UNIV::'var set|"
+  apply (rule card_of_subset_bound)
+   apply (rule SSupp_tvsubst_subset)
+    apply (rule assms Un_bound)+
+  done
+lemma SSupp_Sb_bound:
+  fixes \<rho>2::"'tyvar::var \<Rightarrow> 'tyvar FType"
+  assumes f_prems:
+    "|SSupp TyVar \<rho>2| <o cmin |UNIV::'tyvar set| |UNIV::'var::var set|"
+    "|SSupp TyVar \<rho>1'| <o cmin |UNIV::'tyvar set| |UNIV::'var set|"
+  shows "|SSupp TyVar (tvsubst_FType \<rho>2 \<circ> \<rho>1')| <o cmin |UNIV::'tyvar set| |UNIV::'var set|"
+  apply (rule card_of_subset_bound)
+   apply (rule SSupp_Sb_subset)
+    apply (rule assms Un_bound)+
+  done
 
 pbmv_monad "('tv, 'v) FTerm" and "'tv FType"
   Sbs: tvsubst_FTerm
@@ -665,20 +1087,339 @@ pbmv_monad "('tv, 'v) FTerm" and "'tv FType"
           apply (rule ext)
           apply (rule trans[OF comp_apply])
           apply (rule tvsubst_VVr)
-            apply (assumption | rule cmin_greater card_of_Card_order)+
-  oops
+           apply (assumption | rule cmin_greater card_of_Card_order cmin1 cmin2 | erule ordLess_ordLeq_trans)+
+
+         apply (rule ext)
+         apply (rule trans[OF comp_apply])
+  subgoal for \<rho>'1 \<rho>'2 \<rho>1 \<rho>2 x
+    apply (rule FTerm.fresh_induct_param[of UNIV
+      "\<lambda>t. FTVars (tvsubst_FTerm \<rho>1 \<rho>2 t) \<union> (avoiding_set1 \<rho>1 \<rho>2 \<union> avoiding_set1 \<rho>'1 \<rho>'2) \<union> avoiding_set1 (tvsubst_FTerm \<rho>'1 \<rho>'2 \<circ> \<rho>1) (Sb_FType \<rho>'2 \<circ> \<rho>2)"
+      "\<lambda>t. FVars (tvsubst_FTerm \<rho>1 \<rho>2 t) \<union> avoiding_set2 \<rho>1 \<union> avoiding_set2 \<rho>'1 \<union> avoiding_set2 (tvsubst_FTerm \<rho>'1 \<rho>'2 \<circ> \<rho>1)"
+      _ x, unfolded ball_UNIV, THEN spec, of "\<lambda>t \<rho>. t = \<rho> \<longrightarrow> _ t", THEN mp[OF _ refl]
+    ])
+      apply (((unfold IImsupp_def)[1]), (rule Un_bound UN_bound card_of_Card_order FTerm.FVars_bd_UNIVs FType.FVars_bd_UNIVs
+        SSupp_Sb_bound SSupp_tvsubst_bound[THEN ordLess_ordLeq_trans] SSupp_Sb_bound[THEN ordLess_ordLeq_trans] ordLeq_refl cmin_Card_order
+        var_class.UN_bound var_class.Un_bound cmin1 cmin2 | erule ordLess_ordLeq_trans
+        )+)+
+    apply (rule impI)
+    apply hypsubst
+
+    apply (rule case_split[rotated])
+     apply (subst tvsubst_not_is_VVr[rotated -1])
+           apply assumption+
+        apply (erule Int_subset_empty2)
+        apply (rule subsetI)
+        apply (rule UnI1)
+        apply (rule UnI2)
+        apply (rule UnI1)
+        apply assumption
+        apply (erule Int_subset_empty2)
+        apply (rule subsetI)
+       apply (rule UnI1)
+       apply (rule UnI1)
+       apply (rule UnI2)
+        apply assumption
+      apply assumption
+
+     apply (rule trans)
+      apply (rule tvsubst_not_is_VVr[rotated -1])
+    apply (unfold FTerm_pre.Map_map[symmetric])[1]
+           apply (erule not_is_VVr_Sb[rotated -1])
+            apply (rule supp_id_bound cmin1 cmin2 card_of_Card_order | assumption | erule ordLess_ordLeq_trans)+
+    (* REPEAT_DETERM *)
+    apply (subst FTerm_pre.set_Sb)
+          apply (rule supp_id_bound cmin1 cmin2 card_of_Card_order | assumption | erule ordLess_ordLeq_trans)+
+        apply (subst FTerm_pre.set_map)
+            apply (rule supp_id_bound bij_id)+
+        apply (unfold image_id)
+        apply (erule Int_subset_empty2)
+        apply (rule subsetI)
+        apply (rule UnI1)
+        apply (rule UnI2)
+        apply (rule UnI2)
+        apply assumption
+       apply (subst FTerm_pre.set_Sb FTerm_pre.set_map, (rule supp_id_bound bij_id cmin1 cmin2 card_of_Card_order | erule ordLess_ordLeq_trans)+)+
+       apply (unfold image_id)
+       apply (erule Int_subset_empty2)
+       apply (rule subsetI)
+       apply (rule UnI1)
+       apply (rule UnI2)
+       apply assumption
+      apply (subst noclash_FTerm_def)
+      apply (subst FTerm_pre.set_Sb FTerm_pre.set_map, (rule supp_id_bound bij_id cmin1 cmin2 card_of_Card_order | erule ordLess_ordLeq_trans)+)+
+      apply (unfold image_id)
+      apply (rule conjI)
+       apply (rule Int_subset_empty2)
+        apply assumption
+       apply (rule subsetI)
+       apply (rule UnI1)+
+       apply (subst tvsubst_not_is_VVr, assumption+)
+           apply (erule Int_subset_empty2)
+           apply (rule subsetI)
+           apply (rule UnI1)
+           apply (rule UnI2)
+           apply (rule UnI1)
+           apply assumption
+          apply (erule Int_subset_empty2)
+          apply (rule subsetI)
+           apply (rule UnI1)
+          apply (rule UnI1)
+          apply (rule UnI2)
+          apply assumption
+         apply assumption
+        apply assumption
+    apply (unfold FTerm.FVars_ctor)[1]
+       apply (subst FTerm_pre.set_Sb FTerm_pre.set_map, (rule supp_id_bound bij_id cmin1 cmin2 card_of_Card_order | erule ordLess_ordLeq_trans)+)+
+       apply (unfold image_id)
+       apply (erule UnE)
+        apply (erule UnI1 UnI2 | assumption | rule UnI1)+
+
+
+       apply (rule Int_subset_empty2)
+        apply assumption
+       apply (rule subsetI)
+       apply (rule UnI1)+
+       apply (subst tvsubst_not_is_VVr, assumption+)
+           apply (erule Int_subset_empty2)
+           apply (rule subsetI)
+           apply (rule UnI1)
+           apply (rule UnI2)
+           apply (rule UnI1)
+           apply assumption
+          apply (erule Int_subset_empty2)
+          apply (rule subsetI)
+           apply (rule UnI1)
+          apply (rule UnI1)
+          apply (rule UnI2)
+          apply assumption
+         apply assumption
+        apply assumption
+    apply (unfold FTerm.FVars_ctor)[1]
+       apply (subst FTerm_pre.set_Sb FTerm_pre.set_map, (rule supp_id_bound bij_id cmin1 cmin2 card_of_Card_order | erule ordLess_ordLeq_trans)+)+
+       apply (unfold image_id)
+       apply (erule UnE)
+        apply (erule UnI1 UnI2 | assumption | rule UnI1)+
+
+     apply (subst tvsubst_not_is_VVr)
+           apply (assumption | rule SSupp_tvsubst_bound cmin1 cmin2 card_of_Card_order cmin1 SSupp_Sb_bound | erule ordLess_ordLeq_trans)+
+         apply (erule Int_subset_empty2, rule Un_upper2)+
+       apply assumption
+      apply assumption
+     apply (rule arg_cong[of _ _ FTerm_ctor])
+     apply (unfold FTerm_pre.Map_map[symmetric])[1]
+     apply (subst FTerm_pre.Map_Sb[THEN fun_cong, unfolded comp_def])
+       apply (rule supp_id_bound cmin1 cmin2 card_of_Card_order | erule ordLess_ordLeq_trans)+
+     apply (unfold trans[OF comp_apply[symmetric] FTerm_pre.Map_comp[THEN fun_cong]])[1]
+     apply (rule trans)
+      apply (rule trans[OF comp_apply[symmetric] FTerm_pre.Sb_comp(1)[THEN fun_cong]])
+         apply (rule supp_id_bound cmin1 cmin2 card_of_Card_order | erule ordLess_ordLeq_trans)+
+     apply (unfold id_o o_id)
+     apply (rule arg_cong[of _ _ "Sb_FTerm_pre _ _"])
+    apply (unfold FTerm_pre.Map_map)
+     apply (rule FTerm_pre.map_cong0)
+                      apply (rule supp_id_bound bij_id refl)+
+      apply (unfold atomize_imp[symmetric])
+      apply (rotate_tac -1)
+    apply (erule mp[rotated])
+    subgoal premises prems
+      apply (rule impI)
+      apply (rule trans[OF comp_apply])
+      apply (erule prems)
+      apply (rule refl UNIV_I)+
+      done
+      apply (rotate_tac -1)
+    apply (erule mp[rotated])
+    subgoal premises prems
+      apply (rule impI)
+      apply (rule trans[OF comp_apply])
+      apply (erule prems)
+      apply (rule refl UNIV_I)+
+      done
+
+    apply (unfold isVVr_def)
+    apply (erule exE)
+    apply (rotate_tac -1)
+    apply (erule subst[OF sym])
+    apply (unfold tvsubst_VVr)
+    apply (subst tvsubst_VVr)
+      apply (rule SSupp_tvsubst_bound SSupp_Sb_bound | assumption)+
+    apply (unfold comp_def)
+    apply (rule refl)
+    done
+
+        apply (rule FTerm.FVars_bd)+
+      apply (rule FVars_VVr)+
+    apply (rule FVars_tvsubst; assumption)+
+
+  subgoal premises prems for \<rho>1 \<rho>2 \<rho>1' \<rho>2' t
+    apply (insert prems(5,6))
+    apply (unfold atomize_all atomize_imp)
+    apply (rule FTerm.TT_fresh_induct[of "avoiding_set1 \<rho>1 \<rho>2 \<union> avoiding_set1 \<rho>1' \<rho>2'" "avoiding_set2 \<rho>1 \<union> avoiding_set2 \<rho>1'" _ t])
+    apply (insert prems(1-4))[2]
+apply (((unfold IImsupp_def)[1]), (rule Un_bound UN_bound card_of_Card_order FTerm.FVars_bd_UNIVs FType.FVars_bd_UNIVs cmin_greater
+        var_class.UN_bound var_class.Un_bound cmin1 cmin2 | erule ordLess_ordLeq_trans
+        )+)+
+    apply (unfold atomize_all[symmetric] atomize_imp[symmetric])
+    subgoal premises inner_prems for x
+      apply (insert prems(1-4) inner_prems(3-5))
+    apply (rule case_split[rotated])
+     apply (subst tvsubst_not_is_VVr[rotated -1])
+           apply assumption+
+        apply (erule Int_subset_empty2, rule Un_upper1)+
+    apply assumption
+     apply (subst tvsubst_not_is_VVr[rotated -1])
+           apply assumption+
+        apply (erule Int_subset_empty2, rule Un_upper2)+
+      apply assumption
+     apply (rule arg_cong[of _ _ FTerm_ctor])
+     apply (rule cong'[of _ "map_FTerm_pre id id id id _ _ _" _ "map_FTerm_pre id id id id _ _ _"])
+      apply (rule FTerm_pre.Sb_cong)
+           apply (rule supp_id_bound cmin1 cmin2 card_of_Card_order refl | erule ordLess_ordLeq_trans)+
+        apply (unfold FTerm_pre.Map_map[symmetric] FTerm_pre.Vrs_Map)[1]
+      apply (unfold FTerm_pre.set_Vrs(1-2)[symmetric])[1]
+        apply (rule inner_prems)
+        apply (erule FTerm.FVars_intros)
+
+       apply (rule FTerm_pre.map_cong0)
+                        apply (rule supp_id_bound bij_id refl)+
+      apply (rotate_tac -1)
+      apply (erule distinct_prems_rl[rotated])
+        apply (erule inner_prems)
+      (* REPEAT_DETERM *)
+      apply (rule case_split[of "_ \<in> _", rotated])
+         apply (rule inner_prems)
+         apply (erule FTerm.FVars_intros)
+           apply assumption
+          apply assumption
+         apply (rotate_tac -1)
+         apply (drule disjoint_iff[THEN iffD1, THEN spec, THEN mp, rotated])
+          apply assumption
+         apply (unfold Un_iff de_Morgan_disj)[1]
+      apply (erule conjE)+
+         apply (rule trans)
+          apply (erule notin_SSupp)
+         apply (rule sym)
+         apply (erule notin_SSupp)
+      (* repeated *)
+      apply (rule case_split[of "_ \<in> _", rotated])
+         apply (rule inner_prems)
+         apply (erule FTerm.FVars_intros)
+           apply assumption
+          apply assumption
+         apply (rotate_tac -1)
+         apply (drule disjoint_iff[THEN iffD1, THEN spec, THEN mp, rotated])
+          apply assumption
+         apply (unfold Un_iff de_Morgan_disj)[1]
+      apply (erule conjE)+
+         apply (rule trans)
+          apply (erule notin_SSupp)
+         apply (rule sym)
+         apply (erule notin_SSupp)
+      (* END REPEAT_DETERM *)
+      apply (rotate_tac -1)
+      apply (erule distinct_prems_rl[rotated])
+       apply (erule inner_prems)
+        (* REPEAT_DETERM *)
+        apply (rule inner_prems)
+        apply (erule FTerm.FVars_intros)
+        apply assumption
+        (* repeated *)
+        apply (rule inner_prems)
+        apply (erule FTerm.FVars_intros)
+       apply assumption
+      (* END REPEAT_DETERM *)
+
+      apply (unfold isVVr_def)
+      apply (erule exE)
+      apply (rotate_tac -1)
+      apply (erule distinct_prems_rl[rotated])
+      apply (rotate_tac -1)
+      apply (erule subst[OF sym])
+      apply (unfold tvsubst_VVr)
+      apply (rule inner_prems)
+      apply (rotate_tac -1)
+      apply (erule subst[OF sym])
+      apply (unfold FVars_VVr)
+      apply (rule singletonI)
+      done
+    done
+  done
+print_theorems
+
+mrsbnf "('tv, 'v) FTerm" and "'tv FType"
+   apply (rule ext)
+  subgoal for f1 f2 t
+    apply (rule FTerm.TT_fresh_induct[of "imsupp f1" "imsupp f2" _ t])
+    apply (rule imsupp_supp_bound[THEN iffD2] infinite_UNIV cmin1 cmin2 card_of_Card_order | erule ordLess_ordLeq_trans)+
+    apply (rule case_split[rotated])
+     apply (rule sym)
+     apply (rule trans)
+      apply (erule tvsubst_not_is_VVr[rotated -1])
+          apply (subst SSupp_Inj_comp, rule injI, erule FTerm.Inj_inj[THEN iffD1])
+          apply (assumption)
+         apply ((subst IImsupp_Inj_comp SSupp_Inj_comp IImsupp_def FVars_VVr UN_empty2 Un_empty_left Un_empty_right comp_apply imsupp_absorb,
+          ((rule injI FTerm.Vrs_Inj | erule FTerm.Inj_inj[THEN iffD1] | assumption
+         )+)?)+)[4]
+     apply (rule sym)
+    apply (rule trans)
+     apply (rule FTerm.vvsubst_cctor)
+    apply (rule cmin1 cmin2 card_of_Card_order | erule ordLess_ordLeq_trans)+
+        apply assumption+
+    apply (rule sym)
+     apply (rule arg_cong[of _ _ FTerm_ctor])
+     apply (unfold FTerm_pre.Map_map[symmetric])[1]
+    apply (rule trans)
+      apply (rule trans[OF comp_apply[symmetric] FTerm_pre.map_is_Sb(1)[symmetric, THEN fun_cong]])
+       apply (rule supp_id_bound cmin1 cmin2 card_of_Card_order | erule ordLess_ordLeq_trans)+
+     apply (rule sym)
+    apply (rule FTerm_pre.map_cong0)
+                      apply (rule supp_id_bound bij_id cmin1 cmin2 card_of_Card_order | erule ordLess_ordLeq_trans)+
+          apply (rule refl)
+         apply (unfold FTerm_pre.set_Vrs)[1]
+         apply (subst (asm) eta_compl_free)
+          apply (rule allI)
+          apply (rotate_tac -1)
+          apply (erule contrapos_nn)
+          apply (unfold isVVr_def VVr_def comp_def)[1]
+          apply (rule exI)
+          apply hypsubst
+          apply (rule refl)
+         apply (erule emptyE)
+        apply (rule refl)+
+      apply assumption+
+
+    apply (unfold isVVr_def)[1]
+    apply (erule exE)
+    apply (rotate_tac -1)
+    apply (erule subst[OF sym])
+    apply (rule sym)
+    apply (rule trans)
+     apply (rule tvsubst_VVr)
+      apply (subst SSupp_Inj_comp, rule injI, erule FTerm.Inj_inj[THEN iffD1], assumption+)+
+    apply (subst VVr_def comp_apply)+
+    apply (rule sym)
+    apply (rule trans)
+     apply (rule FTerm.vvsubst_cctor)
+         apply (rule cmin1 cmin2 card_of_Card_order | erule ordLess_ordLeq_trans)+
+       apply (unfold eta_set_empties noclash_FTerm_def)
+       apply (rule Int_empty_left conjI)+
+    apply (rule arg_cong[OF eta_natural'])
+         apply (rule supp_id_bound bij_id cmin1 cmin2 card_of_Card_order | erule ordLess_ordLeq_trans)+
+    done
+  apply (rule FType.map_is_Sb; assumption)
+  done
 
 (* Sugar theorems for substitution *)
 definition Var :: "'v \<Rightarrow> ('tv::var, 'v::var) FTerm" where
-  "Var a \<equiv> FTerm_ctor (Abs_FTerm_pre (Inl a))"
+  "Var a \<equiv> FTerm_ctor (Abs_FTerm_pre (Inl (Inl a)))"
 definition App :: "('tv, 'v) FTerm \<Rightarrow> ('tv, 'v) FTerm \<Rightarrow> ('tv::var, 'v::var) FTerm" where
-  "App t1 t2 \<equiv> FTerm_ctor (Abs_FTerm_pre (Inr (Inl (t1, t2))))"
+  "App t1 t2 \<equiv> FTerm_ctor (Abs_FTerm_pre (Inl (Inr (t1, t2))))"
 definition TyApp :: "('tv, 'v) FTerm \<Rightarrow> 'tv FType \<Rightarrow> ('tv::var, 'v::var) FTerm" where
-  "TyApp t T \<equiv> FTerm_ctor (Abs_FTerm_pre (Inr (Inr (Inl (t, T)))))"
+  "TyApp t T \<equiv> FTerm_ctor (Abs_FTerm_pre ((Inr (Inl (t, T)))))"
 definition Lam :: "'v \<Rightarrow> 'tv FType \<Rightarrow> ('tv, 'v) FTerm \<Rightarrow> ('tv::var, 'v::var) FTerm" where
-  "Lam x T t \<equiv> FTerm_ctor (Abs_FTerm_pre (Inr (Inr (Inr (Inl (x, T, t))))))"
+  "Lam x T t \<equiv> FTerm_ctor (Abs_FTerm_pre (Inr (Inr (Inl (x, T, t)))))"
 definition TyLam :: "'tv \<Rightarrow> ('tv, 'v) FTerm \<Rightarrow> ('tv::var, 'v::var) FTerm" where
-  "TyLam a t \<equiv> FTerm_ctor (Abs_FTerm_pre (Inr (Inr (Inr (Inr (a, t))))))"
+  "TyLam a t \<equiv> FTerm_ctor (Abs_FTerm_pre (Inr (Inr (Inr (a, t)))))"
 
 lemma FTerm_subst:
   fixes f1::"'v \<Rightarrow> ('tv::var, 'v::var) FTerm" and f2::"'tv \<Rightarrow> 'tv FType"
@@ -705,13 +1446,13 @@ lemma FTerm_subst:
       apply (rule notI)
       apply (erule exE conjE)+
       apply (unfold map_FTerm_pre_def comp_def Abs_FTerm_pre_inverse[OF UNIV_I] map_sum.simps prod.map_id
-      Abs_FTerm_pre_inject[OF UNIV_I UNIV_I]
+      Abs_FTerm_pre_inject[OF UNIV_I UNIV_I] sum.inject
       )[1]
       apply (rotate_tac -1)
       apply (erule contrapos_pp)
       apply (rule sum.distinct)
      apply (unfold map_FTerm_pre_def comp_def Abs_FTerm_pre_inverse[OF UNIV_I] map_sum.simps prod.map_id
-      Abs_FTerm_pre_inject[OF UNIV_I UNIV_I] Sb_FTerm_pre_def id_def map_prod_simp
+      Abs_FTerm_pre_inject[OF UNIV_I UNIV_I] Sb_FTerm_pre_def id_def map_prod_simp bmv_defs
       )[1]
      apply (rule refl)
 
